Reorganize tactics hierarchy.

rocq-osiris/theories/proofmode/specifications.v
@@ -1,18 +1,13 @@
-From iris.proofmode Require Import base proofmode classes.
-From iris.base_logic.lib Require Import fancy_updates.
-From iris.bi Require Import weakestpre.
-From iris.prelude Require Import options.
-Import uPred.
+From iris.proofmode Require Import proofmode.
 
-From osiris Require Import base.
-From osiris.lang Require Import lang.
-From osiris.semantics Require Import semantics.
+From osiris.lang Require Import encode type_nel.
 From osiris.program_logic Require Import program_logic.
+
+From osiris.tactics Require Import utils iris_bindings.
+From osiris.proofmode Require Import equality.
 
 (* --------------------------------------------------------------------------*)
 (* The following part defines module specifications. *)
-
-From iris.base_logic Require Import iprop.
 
 Lemma lookup_name_nil name :
   lookup_name [] name = None.
@@ -50,12 +45,17 @@ Section Modules.
   Definition path_spec `{Encode A} (p : path) (spec : A → iProp Σ) (η : env) : iProp Σ :=
     ∃ x, ⌜lookup_path η p = Some #x⌝ ∗ spec x.
 
-  Definition var_spec `{Encode A} (name : var) (spec : A → iProp Σ) (η : env) : iProp Σ :=
+  (* Specification over a variable name. *)
+
+  Definition in_env `{Encode A} (name : var) (spec : A → iProp Σ) (η : env) : iProp Σ :=
     ∃ x, ⌜lookup_name η name = Some #x⌝ ∗ spec x.
 
+  Definition pure_in_env `{Encode A} (name : var) (spec : A → Prop) (η : env) : Prop :=
+    ∃ x, lookup_name η name = Some #x ∧ spec x.
+
   Lemma var_spec_app `{Encode A} x (Φ : A → iProp Σ) δ η :
-    var_spec x Φ δ -∗
-    var_spec x Φ (δ ++ η).
+    in_env x Φ δ -∗
+    in_env x Φ (δ ++ η).
   Proof.
     iIntros "(% & % & $)".
     iPureIntro.
@@ -63,45 +63,57 @@ Section Modules.
   Qed.
 
   Lemma var_spec_mono `{Encode A} {Φ : A → iProp Σ} (Φ' : A → iProp Σ) x η :
-    var_spec x Φ' η -∗
+    in_env x Φ' η -∗
     (∀ a, Φ' a -∗ Φ a) -∗
-    var_spec x Φ η.
+    in_env x Φ η.
   Proof.
     iIntros "(%a & % & HΦ') Hmono".
     iExists a. iSplit; [ iPureIntro; assumption | ].
     iApply ("Hmono" with "HΦ'").
   Qed.
 
-  Record enc_spec :=
-    Spec
+  Record enc_spec {PROP : Type} :=
+    has_spec
       {
         res_type : Type;
         res_type_enc : Encode res_type;
         name : var;
-        spec : res_type → iProp Σ;
+        spec : res_type → PROP;
       }.
   (* Make it so [enc_spec] displays as [Spec name Φ]. *)
-  Global Arguments Spec {_ _}.
+  Global Arguments enc_spec {_}.
+  Global Arguments res_type {_}.
+  Global Arguments res_type_enc {_}.
+  Global Arguments name {_}.
+  Global Arguments spec {_}.
+  Global Arguments has_spec {_ _ _}.
   Global Add Printing Constructor enc_spec.
 
   Instance dom_env : Dom (env) (gset var) := λ η, list_to_set (η.*1).
 
-  Definition context (specs : list enc_spec) d : env → iProp Σ :=
+  Definition context (specs : list (@enc_spec (iProp Σ))) d : env → iProp Σ :=
     λ η, (⌜dom η = d⌝ ∗
            [∗ list] s ∈ specs,
-            @var_spec s.(res_type) s.(res_type_enc) s.(name) (λ res, □ s.(spec) res) η)%I.
+            @in_env s.(res_type) s.(res_type_enc) s.(name) (λ res, □ s.(spec) res) η)%I.
+
+  Definition pure_context (specs : list (@enc_spec Prop)) d : env → Prop :=
+    λ η, dom η = d ∧
+         Forall (λ s,
+                   @pure_in_env s.(res_type) s.(res_type_enc) s.(name) s.(spec) η) specs.
 
   Global Instance context_pers specs d η : Persistent (context specs d η).
   Proof. apply _. Qed.
 
-  Check
-  context [
-      Spec "+" (λ add, iSpec τ[Z; Z] add (λ i j m, imp m {{ λ n, ⌜(n = i + j)%Z⌝ }})%I);
-      Spec "-" (λ sub, iSpec τ[Z; Z] sub (λ i j m, imp m {{ λ n, ⌜(n = i - j)%Z⌝ }})%I)
-    ] {["+";"-";"*"]}.
+  (*
+    Check
+    context [
+       has_spec "+" (λ add, iSpec τ[Z; Z] add (λ i j m, imp m {{ λ n, ⌜(n = i + j)%Z⌝ }})%I);
+       has_spec "-" (λ sub, iSpec τ[Z; Z] sub (λ i j m, imp m {{ λ n, ⌜(n = i - j)%Z⌝ }})%I)
+     ] {["+";"-";"*"]}.
+   *)
 
   Lemma extract_context `{Encode A} {η} xs ys d name (spec : A → iProp Σ) :
-    context (xs ++ [Spec name spec] ++ ys) d η -∗ var_spec name spec η.
+    context (xs ++ [has_spec name spec] ++ ys) d η -∗ in_env name spec η.
   Proof.
     unfold context.
     iIntros "(%Hdom & Hspecs)".
@@ -112,12 +124,12 @@ Section Modules.
     iIntros (res) "#Hspec'". iApply "Hspec'".
   Qed.
 
-  (* We immediately reduce [path_spec] to [var_spec] if the path is a singleton. *)
+  (* We immediately reduce [path_spec] to [in_env] if the path is a singleton. *)
 
   Lemma path_spec_singleton `{Encode A} name (Φ : A → iProp Σ) η :
-    var_spec name Φ η -∗ path_spec [name] Φ η.
+    in_env name Φ η -∗ path_spec [name] Φ η.
   Proof.
-    unfold var_spec.
+    unfold in_env.
     iIntros "(%x & Hlookup & HΦ)".
     iExists x. simpl. iFrame.
   Qed.
@@ -126,7 +138,7 @@ Section Modules.
      at the head of the path. *)
 
   Lemma path_spec_cons {A : Type} `{Encode A} {Φ : A → iProp Σ} {η x p} mspec :
-    var_spec x mspec η -∗
+    in_env x mspec η -∗
     (∀ (δ : env), mspec δ -∗ path_spec p Φ δ) -∗
     path_spec (x :: p) Φ η.
   Proof.
@@ -145,8 +157,8 @@ Section Modules.
 
   Lemma var_spec_cons {A : Type} `{Encode A} {Φ : A → iProp Σ} {η v} x y :
     (x =? y)%string = false →
-    var_spec x Φ η -∗
-    var_spec x Φ ((y, v) :: η).
+    in_env x Φ η -∗
+    in_env x Φ ((y, v) :: η).
   Proof.
     iIntros (Hneq) "(%a & %Hlookup & $)".
     iPureIntro.
@@ -160,7 +172,7 @@ Section Modules.
   Lemma var_spec_here {A : Type} `{Encode A} {Φ : A → iProp Σ} {η v} x y :
     (x =? y)%string = true →
     Φ v -∗
-    var_spec x Φ ((y, #v) :: η).
+    in_env x Φ ((y, #v) :: η).
   Proof.
     iIntros (Heq) "$".
     iPureIntro.
@@ -174,8 +186,8 @@ Section Modules.
   Lemma var_spec_app_r `{Encode A} {Φ : A → iProp Σ} {η x} δ d mspec :
     x ∉ d →
     context mspec d δ -∗
-    var_spec x Φ η -∗
-    var_spec x Φ (δ ++ η).
+    in_env x Φ η -∗
+    in_env x Φ (δ ++ η).
   Proof.
     iIntros (Hnin) "(%Hdom & _) Hη".
     iInduction δ as [| [y v] δ ] "IH" forall (d Hnin Hdom).
@@ -199,8 +211,8 @@ Section Modules.
      fragment. *)
 
   Lemma var_spec_app_l `{Encode A} {Φ : A → iProp Σ} {η x} δ d xs ys :
-    context (xs ++ [Spec x Φ] ++ ys) d δ -∗
-    var_spec x Φ (δ ++ η).
+    context (xs ++ [has_spec x Φ] ++ ys) d δ -∗
+    in_env x Φ (δ ++ η).
   Proof.
     iIntros "Hcontext".
     iPoseProof (extract_context with "Hcontext") as "Hspec".
@@ -210,9 +222,9 @@ Section Modules.
   (* We can pick out the right specification from a context. *)
 
   Lemma var_spec_context `{Encode A} {Φ : A → iProp Σ} {x} δ d specs :
-    Spec x Φ ∈ specs →
+    has_spec x Φ ∈ specs →
     context specs d δ -∗
-    var_spec x Φ δ.
+    in_env x Φ δ.
   Proof.
     iIntros (Hin) "Hcontext".
     apply list_elem_of_split in Hin as (l1 & l2 & ->).
@@ -220,10 +232,10 @@ Section Modules.
   Qed.
 
   Lemma var_spec_context_mono `{Encode A} {Φ : A → iProp Σ} Φ' {x} δ d specs :
-    Spec x Φ' ∈ specs →
+    has_spec x Φ' ∈ specs →
     context specs d δ -∗
     (∀ a, Φ' a -∗ Φ a) -∗
-    var_spec x Φ δ.
+    in_env x Φ δ.
   Proof.
     iIntros (Hin) "Hcontext Hmono".
     apply list_elem_of_split in Hin as (l1 & l2 & ->).
@@ -253,6 +265,164 @@ Section Modules.
 
 End Modules.
 
+(* --------------------------------------------------------------------------*)
+(* Implementing the [imp_path] tactic. *)
+
+From Ltac2 Require Import Ltac2 Printf.
+
+Ltac2 get_env_spec (η : constr) :=
+  let (pers_hyps, spat_hyps) := get_iris_hyps () in
+  let rec go env :=
+    lazy_match! env with
+    | environments.Enil =>
+        Control.zero (Tactic_failure
+                        (Some (fprintf "Could not find [context] specification for environment %t" η)))
+    | environments.Esnoc ?env ?name ?prop =>
+        match! prop with
+        | specifications.context ?_specs ?_domain ?δ =>
+            if Constr.equal η δ then
+              name
+            else
+              go env
+        | ?_spec ?δ =>
+            if Constr.equal η δ then
+              name
+            else
+              go env
+        | _ => go env
+        end
+    end
+  in
+  Control.plus
+    (fun _ => go pers_hyps)
+    (fun _ => go spat_hyps).
+
+Ltac2 var_spec_cons () :=
+  iApply var_spec_cons; Control.focus 1 1 (fun _ => reflexivity).
+
+Ltac2 var_spec_here () :=
+  iApply var_spec_here; Control.focus 1 1 (fun _ => reflexivity).
+
+Ltac2 var_spec_app_r (hyp : constr) :=
+  iApply (var_spec_app_r with $hyp);
+  Control.focus 1 1 (fun _ => complete (fun _ => ltac1:(set_solver))).
+
+Ltac2 var_spec_app () :=
+  iApply var_spec_app.
+
+Ltac2 var_spec_context hyp :=
+  Control.plus
+    (fun _ =>
+       iApply (var_spec_context with $hyp);
+       complete (fun _ => repeat constructor))
+    (fun _ =>
+       iApply (var_spec_context_mono with $hyp) >
+         [  complete (fun _ => repeat constructor) | auto ]).
+
+Ltac2 rec solve_var_spec () :=
+  lazy_match! get_iris_goal () with
+  | in_env ?name ?_spec ?env =>
+      match! env with
+      | (?name', ?_val) :: _ =>
+          if Constr.equal name name' then
+            var_spec_here ()
+          else
+            (var_spec_cons ();
+             Control.enter solve_var_spec)
+      | ?δ ++ ?_η =>
+          Control.plus
+            (fun _ =>
+               let spec_name := get_env_spec δ in
+               var_spec_app_r spec_name;
+               last solve_var_spec)
+            (fun _ =>
+               var_spec_app ();
+               solve_var_spec ())
+      | ?η =>
+          Control.plus
+            (fun _ => iAssumption)
+            (fun _ =>
+               Control.plus
+                 (fun _ =>
+                    let spec_name := get_env_spec η in
+                    var_spec_context spec_name)
+                 (fun _ =>
+                    Control.zero (Tactic_failure
+                                    (Some (fprintf "Could not solve goal [var_spec %t _ %t]" name env)))))
+      end
+  | _ => Control.zero (Tactic_failure (Some (fprintf "Expected goal to be [path_spec]")))
+  end.
+
+Ltac2 Type detected_path :=
+  [ | Psingleton
+    | Pcons ].
+
+Ltac2 rec path_spec_to_var_spec () :=
+  lazy_match! get_iris_goal () with
+  | path_spec ?path ?_spec ?_env =>
+      match! path with
+      | [ _ ] =>
+          iApply path_spec_singleton;
+          Psingleton
+      | _ =>
+          iApply path_spec_cons;
+          Pcons
+      end
+  | _ => Control.zero (Tactic_failure (Some (fprintf "Expected goal to be [path_spec]")))
+  end.
+
+Ltac2 rec solve_path_spec () :=
+  match path_spec_to_var_spec () with
+  | Psingleton => solve_var_spec ()
+  | Pcons =>
+      Control.focus 1 1 (fun _ => complete solve_var_spec);
+      let hyp_name := iFresh "Hpath" in
+      iIntros ("% #" ++ $hyp_name)%string;
+      solve_path_spec ()
+  end.
+
+Ltac2 solve_eq_goal () :=
+  lazy_match! get_iris_goal () with
+  | (⌜_ = _⌝)%I => ltac1:(equality)
+  | ?spec ?x =>
+      match Constr.Unsafe.kind spec with
+      | Constr.Unsafe.Evar _ _ =>
+          let prop := '(λ x,⌜x=$x⌝)%I in
+          try_complete (fun _ => Std.unify spec prop; auto)
+      | _ => ()
+      end
+  end.
+
+Ltac2 imp_path_tac () :=
+  iApply imp_EPath_spec;
+  solve_path_spec ().
+
+Ltac2 Notation "imp_path" :=
+  (* Resolve the path. *)
+  imp_path_tac ();
+  (* If there is a goal remaining. *)
+  Control.enter
+    (fun _ =>
+       if empty_spatial_env () then
+         (* If there are no resources, first try to solve the goal as an equality. *)
+         solve_eq_goal ();
+         (* If that failed, try to frame the persistent resources. *)
+         Control.enter (fun _ => iFrame "#")
+       else
+         try_complete (fun _ => iFrame)).
+Tactic Notation "imp_path" := ltac2:(imp_path).
+
+Ltac2 Notation "imp_path_eq" :=
+  imp_path_tac (); solve_eq_goal ().
+Tactic Notation "imp_path_eq" := ltac2:(imp_path_eq).
+
+(* --------------------------------------------------------------------------*)
+(* Testing the [imp_path] tactic. *)
+
+From iris.proofmode Require Import ltac_tactics.
+
+Set Default Proof Mode "Classic".
+
 Section TacticTests.
 
   Context `{!osirisGS Σ}.
@@ -260,9 +430,12 @@ Section TacticTests.
   Local Open Scope Z.
 
   (* We define a short program, [e]:
+     ```
      let x = 2 in
      let y = z in
-     Module1.add (Module2.Module3.sub y x) x *)
+     Module1.add (Module2.Module3.sub y x) x
+     ```
+   *)
 
   Definition e :=
     ELet [Binding (PVar "x") (EInt 2)] (
@@ -285,65 +458,39 @@ Section TacticTests.
   Definition add_spec add : iProp Σ := □ iSpec τ[Z;Z] add (λ (i j : Z) m, imp m {{ λ k, ⌜(k = i + j)%Z⌝ }})%I.
   Definition sub_spec sub : iProp Σ := □ iSpec τ[Z;Z] sub (λ (i j : Z) m, imp m {{ λ k, ⌜(k = i - j)%Z⌝ }})%I.
 
-  Definition module3_spec := context [Spec "sub" sub_spec] {["sub"]}.
-  Definition module2_spec := context [Spec "Module3" module3_spec] {["Module3"; "some"; "other"; "stuff"]}.
+  Definition module3_spec η := context [has_spec "sub" sub_spec] {["sub"]} η.
+  Definition module2_spec η := context [has_spec "Module3" module3_spec] {["Module3"; "some"; "other"; "stuff"]} η.
 
   Lemma example_proof δ η :
-    var_spec "z" (λ (i : Z), ⌜i > 0⌝) η -∗
-    context [Spec "Module1" (context [Spec "some_other_val" (λ (_ : val), True);
-                                      Spec "add" add_spec] {["add"]})] {["Module1"]} δ -∗
-    context [Spec "Module2" module2_spec] {["Module2"]} η -∗
+    in_env "z" (λ (i : Z), ⌜i > 0⌝) η -∗
+    context [has_spec
+               "Module1"
+               (context [has_spec "some_other_val" (λ (_ : val), True);
+                         has_spec "add" add_spec] {["some_other_val";"add"]})
+      ] {["Module1"]} δ -∗
+    context [has_spec "Module2" module2_spec] {["Module2";"z"]} η -∗
     imp (eval (δ ++ η) e) {{ λ (i : Z), ⌜i > 0⌝ }}.
   Proof.
     iIntros "#zspec #δspec #ηspec".
-    iApply (imp_ELet_var (B:=Z)). { iApply imp_EInt. }
+    (* TODO: imp_let tactic which instantiates
+       the return type of the left member with an evar. *)
+    evar(B:Type).
+    evar(HB:Encode B).
+    iApply (imp_ELet_var (B:=B)). { iApply imp_EInt. }
+    subst B HB.
     iIntros (? ->).
     iApply (imp_ELet_var (B:=Z)).
-    { iApply imp_EPath_spec.
-      iApply path_spec_singleton.
-      iApply var_spec_cons; first auto.
-      iApply (var_spec_app_r with "δspec"). { set_solver. }
-      iAssumption. }
-    iIntros (y) "%yspec".
+    { imp_path. }
+    iIntros (z) "%yspec".
     iApply (imp_EApp τ[Z;Z]).
-    { iApply imp_EPath_spec.
-      iApply path_spec_cons.
-      { iApply var_spec_cons; first auto.
-        iApply var_spec_cons; first auto.
-        iApply var_spec_app.
-        iApply (var_spec_context_mono with "δspec"); [ repeat constructor | auto ]. }
-      iIntros (?) "#module1spec".
-      iApply path_spec_singleton.
-      iApply (var_spec_context_mono with "module1spec"); first repeat constructor.
-      auto. }
+    { imp_path. }
     { iApply (imp_EApp τ[Z;Z]).
-      { iApply imp_EPath_spec.
-        iApply path_spec_cons.
-        { iApply var_spec_cons; first auto.
-          iApply var_spec_cons; first auto.
-          iApply (var_spec_app_r with "δspec"). { set_solver. }
-          iApply (var_spec_context with "ηspec"). repeat constructor. }
-        iIntros (?) "#module2spec".
-        iApply path_spec_cons. { iApply (var_spec_context with "module2spec"). repeat constructor. }
-        iIntros (?) "#module3spec".
-        iApply path_spec_singleton.
-        iApply (var_spec_context_mono with "module3spec"); [ repeat constructor | auto ]. }
-      { iApply imp_EPath_spec.
-        iApply path_spec_singleton.
-        iApply var_spec_here; first auto.
-        instantiate (1:=(λ y',⌜y'=y⌝)%I). auto. }
-      { iApply imp_EPath_spec.
-        iApply path_spec_singleton.
-        iApply var_spec_cons; first auto.
-        iApply var_spec_here; first auto.
-        instantiate (1:=(λ y',⌜y'=2⌝)%I). auto. }
+      { imp_path. }
+      { imp_path. }
+      { imp_path. }
       iIntros (??) "-> -> %m Hm !>".
       iApply "Hm". }
-    { iApply imp_EPath_spec.
-      iApply path_spec_singleton.
-      iApply var_spec_cons; first auto.
-      iApply var_spec_here; first auto.
-      instantiate (1:=(λ y',⌜y'=2⌝)%I). auto. }
+    { imp_path. }
     iIntros (??) "-> -> %m Hm !>".
     iApply (imp_mono_ret with "Hm").
     iIntros (x ->). iPureIntro.
