rocq-osiris/theories/proofmode/ewp_tactics.v
@@ -12,75 +12,13 @@ From osiris.semantics Require Import semantics.
 From osiris.program_logic Require Import program_logic.
 From osiris.proofmode Require Import specifications pure_tactics.
 
-From Ltac2 Require Import Ltac2.
-
-(* -------------------------------------------------------------------------- *)
-
-(** *Ltac2 bindings for Iris Proofmode tactics *)
-
-Ltac2 iapply (lem : constr) (sel : constr option) :=
-  match sel with
-  | None => ltac1:(lem |- iApply lem) (Ltac1.of_constr lem)
-  | Some sel =>
-      ltac1:(lem sel |- iApply (lem with sel))
-              (Ltac1.of_constr lem) (Ltac1.of_constr sel)
-  end.
-
-Ltac2 Notation "iApply" "(" lem(constr) "with" sel(constr) ")" := iapply lem (Some sel).
-Ltac2 Notation "iApply" lem(constr) := iapply lem None.
-
-Ltac2 iintros (pat : constr) :=
-  ltac1:(pat |- iIntros pat) (Ltac1.of_constr pat).
-
-Ltac2 Notation "iIntros" pat(constr) := iintros pat.
-
-Ltac2 iFrame () := ltac1:(iFrame).
-Ltac2 Notation "iFrame" := iFrame ().
-
-Ltac2 iSplit () := ltac1:(iSplit).
-Ltac2 Notation "iSplit" := iSplit ().
-
-Ltac2 iSplitL (selpat : constr) := ltac1:(selpat |- iSplitL selpat) (Ltac1.of_constr selpat).
-Ltac2 Notation "iSplitL" pat(constr) := iSplitL pat.
-
-Ltac2 iSplitR (selpat : constr) := ltac1:(selpat |- iSplitR selpat) (Ltac1.of_constr selpat).
-Ltac2 Notation "iSplitR" pat(constr) := iSplitR pat.
-
-Ltac2 iDestruct (lem : constr) (pat : constr) :=
-  ltac1:(lem pat |- iDestruct (lem) as pat)
-    (Ltac1.of_constr lem) (Ltac1.of_constr pat).
-Ltac2 Notation "iDestruct" "(" lem(constr) ")" "as" pat(constr) := iDestruct lem pat.
-
-Ltac2 iRevert (h : constr) :=
-  ltac1:(h |- iRevert h) (Ltac1.of_constr h).
-Ltac2 Notation "iRevert" h(constr) := iRevert h.
-
-Ltac2 iPureIntro () := ltac1:(iPureIntro).
-Ltac2 Notation "iPureIntro" := iPureIntro ().
-
-Ltac2 iStartProof () := ltac1:(iStartProof).
-Ltac2 Notation "iStartProof" := iStartProof ().
-
-Ltac2 iModIntro () := ltac1:(iModIntro).
-Ltac2 Notation "iModIntro" := iModIntro ().
-
-Tactic Notation "iIntros_RET" :=
-  iIntros ([|]); [ simpl | iIntros "[]" ].
-Tactic Notation "iIntros_RET" constr(pat) :=
-  iIntros ([|]); [ simpl; iIntros pat | iIntros "[]" ].
-Tactic Notation "iIntros_RET" "(" simple_intropattern(v) ")" :=
-  iIntros ([ v |]); [ simpl | iIntros "[]" ].
-Tactic Notation "iIntros_RET" "(" simple_intropattern(v) ")" constr(pat) :=
-  iIntros ([ v |]); [ simpl; iIntros pat | iIntros "[]" ].
-
+From osiris.tactics Require Import tactics.
 
 (** *Utility *)
 
 Section helper_lemmas.
 
 Context `{!osirisGS Σ}.
-
-Set Default Proof Mode "Classic".
 
 Lemma bi_sep_intro (P Q : iProp Σ) :
   P -∗
@@ -99,95 +37,17 @@ Qed.
 
 End helper_lemmas.
 
-Ltac2 all (tac : unit -> unit) :=
-  Control.extend [] tac [].
+From Ltac2 Require Import Ltac2.
 
-(* [iris_goal] gives the current iris goal. *)
-
-Ltac2 iris_goal () : constr :=
-  lazy_match! goal with
-  | [ |- environments.envs_entails _ ?g ] => g
-  | [ |- _ ] =>
-      Control.throw
-        (Tactic_failure
-           (Some
-              (Message.of_string "Expected an iris proofmode goal")))
-  end.
-
-Ltac2 iris_env () : constr :=
-  lazy_match! goal with
-  | [ |- environments.envs_entails ?env _ ] => env
-  | [ |- _ ] =>
-      Control.throw
-        (Tactic_failure
-           (Some
-              (Message.of_string "Expected an iris proofmode goal")))
-  end.
-
-(* Given a constr of the form [▷^n c] (where [n] might equal 0),
-   [strip_laters] returns [c]. *)
-
-Ltac2 rec strip_laters (g : constr) :=
-  lazy_match! g with
-  | bi_later ?c => strip_laters c
-  | _ => g
-  end.
 
 Create HintDb osiris.
+
+Set Default Proof Mode "Classic".
 
 (* Some hints used for resolving [repr] expressions *)
 Global Hint Rewrite eq_repr_repr sub_repr_repr mul_repr_repr: osiris.
 Global Hint Extern 1 (representable _) => representable : osiris.
 Global Hint Unfold val_as_int : osiris.
-
-(** *"WP" tactics
-
-  These tactics operate on [WP] goals are Hoare-style;
-
-  All tactics that are not "Hoare-style" are internal and should not be exposed
-  to the user. *)
-
-(** [uchange A with B] is an untyped version of [change A with B]: it guesses
-  types in [A = B] instead of trying to type [A] and [B] independently *)
-Tactic Notation "uchange" uconstr(A) "with" uconstr(B) :=
-  let Heq := fresh "Heq" in
-  assert (A = B) as Heq;
-  [ | rewrite Heq; clear Heq ];
-  [ reflexivity | ].
-
-(** Use [iExactEq "H"] if the Iris goal is provably equal, but not convertible
-   to, an Iris hypothesis ["H" : hyp], which will replace your [goal] with
-   [⌜goal = hyp⌝] *)
-Tactic Notation "iExactEq" constr(irisHyp) :=
-  match goal with
-  | |- envs_entails ?Δ ?goal =>
-    match Δ with
-    | context[Esnoc _ (INamed irisHyp) ?hyp] =>
-      iAssert ⌜goal = hyp⌝%I as %->; [ | iApply irisHyp ]
-    end
-  end.
-
-(** Use [iExactEq "H" n] to perform [iPureIntro] and n [f_equal]s just after *)
-Tactic Notation "iExactEq" constr(irisHyp) int_or_var(n) :=
-  iExactEq irisHyp; iPureIntro; do n f_equal.
-
-(* -------------------------------------------------------------------------- *)
-
-(* If anything has been added to the hint data base of [osiris], using
-    [Hint Rewrite] or [Hint Extern], then apply the automation. *)
-Ltac Auto :=
-  autorewrite with osiris;
-  auto with osiris.
-
-(* -------------------------------------------------------------------------- *)
-(* If the branch guard in [if _ then _ else _] can be resolved, we can decide
-   which branch to take. *)
-Ltac IfThenElse :=
-  match goal with
-  | |- envs_entails _ (ewp_def _ (if ?b then _ else _) _ _) =>
-      try (assert (b = false) as ->; first done);
-      try (assert (b = true) as ->; first done)
-  end.
 
 (* -------------------------------------------------------------------------- *)
 
@@ -199,36 +59,22 @@ Ltac IfThenElse :=
 Global Hint Extern 0 (envs_entails _ (bi_forall (fun _ : void => _))) => iIntros (?)
 ; try done : core.
 
-(* -------------------------------------------------------------------------- *)
-
-(** *Fetching specifications of functions*)
-
-(* Returns [spec] for the first occurrence of [(name, spec)] in [specs] *)
-(* Ltac spec_of_name specs name := *)
-(*   match specs with *)
-(*   | (name, ?spec) :: _ => constr:(spec) *)
-(*   | _ :: ?l => spec_of_name l name *)
-(*   end. *)
-
-(* From [env_has_pspecs Λ η], add to Coq hypotheses [lookup_name η x = ret v]
-   and the corresponding specification for [x] *)
-(* Tactic Notation "get_spec" constr(name) "as" simple_intropattern(Hv) := *)
-(*   match goal with *)
-(*     He : env_has_pspecs ?specs ?η |- _ => *)
-(*       let spec := spec_of_name specs name in *)
-(*       edestruct (env_has_pspecs_find name spec He) as Hv; *)
-(*       [ repeat first [ left; reflexivity | right ] (* solving List.In *) *)
-(*       | ] *)
-(*   end. *)
-
 (** *Set postcondition *)
 
 (* Force a postcondition, for example when the postcondition is an evar and one
    wants to perform an induction *)
-Tactic Notation "set_postcondition" uconstr(φ) :=
-  match goal with
-  | |- envs_entails _ (ewp_def ?E ?m ?Ψ ?Φ) => assert (Φ = φ) as -> by reflexivity
+Ltac2 set_postcondition_tac (φ : constr) : unit :=
+  lazy_match! get_iris_goal () with
+  | impure ?_e ?_m ?_Ψ ?_ζ ?Φ =>
+      Std.unify Φ φ
+  | _ => Control.zero
+           (Tactic_failure (Some (Message.of_string "Expected goal of the form [imp m @ E <|Ψ|> ⟨⟨ ζ ⟩⟩ {{ Φ }}]")))
   end.
+Ltac2 Notation "set_postcondition" φ(constr) := set_postcondition_tac φ.
+Tactic Notation "set_postcondition" uconstr(φ) :=
+  let tac := ltac2:(φ |- set_postcondition_tac (Option.get (Ltac1.to_constr φ))) in
+  tac φ.
+
 
 (* -------------------------------------------------------------------------- *)
 
@@ -245,118 +91,9 @@ Ltac prove_handler_spec :=
 
 (** *Entering and Skipping Handler Branches *)
 
-(* Takes an iris environment and returns an ltac list containing the
-   idents present in the environment. *)
-
-Ltac2 rec to_ident_list (env : constr) (acc : constr list) :=
-  lazy_match! env with
-  | environments.Enil => acc
-  | environments.Esnoc ?env ?h _ =>
-      to_ident_list env (h :: acc)
-  end.
-
-Ltac2 all_intuitionistic_hyps () :=
-  let env := iris_env () in
-  lazy_match! env with
-  | environments.Envs ?intuitionistic_env _ _ =>
-      to_ident_list intuitionistic_env []
-  end.
-
-Ltac2 all_spatial_hyps () :=
-  let env := iris_env () in
-  lazy_match! env with
-  | environments.Envs _ ?spatial_env _ =>
-      to_ident_list spatial_env []
-  end.
-
-(* [conj_hyps] makes a single conjunction from list of iris hypotheses.
-   The new conjunction has the name of the head of the original list. *)
-
-Ltac2 rec conj_hyps (hyps : constr list) :=
-  match hyps with
-  | [] | [_] => ()
-  | h1 :: (h2 :: hyps) =>
-      ltac1:(h1 h2 |-
-      let h := iFresh in
-      iPoseProof (bi_sep_intro) as h;
-      iSpecialize (h with h1);
-      iSpecialize (h with h2);
-      iRename h into h1) (Ltac1.of_constr h1) (Ltac1.of_constr h2);
-      conj_hyps (h1 :: hyps)
-  end.
-
-(* Given a list of hypotheses that has been turned into a single
-   conjuction, [unconj_hyps] reestablishes the original hypotheses. *)
-
-Ltac2 rec unconj_hyps_aux (hyp_name : constr) (hyps : constr list) :=
-  match hyps with
-  | [] | [_] => ()
-  | h1 :: t =>
-      ltac1:(h1 hyp_name |-
-      _iDestruct0 hyp_name
-        (intro_patterns.IList [[intro_patterns.IIdent hyp_name;
-                                intro_patterns.IIdent h1]]))
-              (Ltac1.of_constr h1) (Ltac1.of_constr hyp_name);
-      unconj_hyps_aux hyp_name t
-  end.
-
-Ltac2 unconj_hyps (hyps : constr list) :=
-  match hyps with | [] => () | hyp_name :: _ =>
-  let hyps := List.rev hyps in
-  unconj_hyps_aux hyp_name hyps
-  end.
-
-(* [revert_intuitionistic] takes a list of persisent (intuitionistic)
-   hypotheses and turns them into hypotheses of the form ["H" : □ P]. *)
-
-Ltac2 rec revert_intuitionistic (hyps : constr list) :=
-  match hyps with
-  | [] => ()
-  | h :: t =>
-      iRevert $h; iIntros $h; revert_intuitionistic t
-  end.
-
-(* [unrevert_intuitionistic] takes a list of hypotheses of the form
-   ["H" : □ P] and (re)introduces them into the intuitionistic
-   environment. *)
-
-Ltac2 rec unrevert_intuitionistic (hyps : constr list) :=
-  match hyps with
-  | [] => ()
-  | h :: t =>
-      iRevert $h;
-      ltac1:(h |- _iIntros0 (intro_patterns.IIntuitionistic (intro_patterns.IIdent h)))
-      (Ltac1.of_constr h);
-      unrevert_intuitionistic t
-  end.
-
-(* Given a goal of the form [(□ H1 ∗ ⋯ ∗ □ Hn) ∗ (P1 ∗ ⋯ ∗ Pm) -∗ G],
-   a list of the persistent hypotheses [H1, ⋯, Hn], and a list of the
-   spatial hypotheses [P1, ⋯, Pm], introduce the hypotheses. *)
-
-Ltac2 reintroduce_env (intuitionistic_hyps : constr list) (spatial_hyps : constr list) :=
-  match intuitionistic_hyps with
-  | h1 :: _ =>
-      iIntros $h1;
-      match spatial_hyps with
-      | h2 :: _ => unconj_hyps [h1; h2]
-      | _ => ()
-      end
-  | _ =>
-      match spatial_hyps with
-      | h2 :: _ =>
-          iIntros $h2
-      | _ => ()
-      end
-  end;
-  unconj_hyps intuitionistic_hyps;
-  unrevert_intuitionistic intuitionistic_hyps;
-  unconj_hyps spatial_hyps.
-
 Ltac2 do_iintros () :=
   try (iModIntro);
-  let igoal := iris_goal () in
-  lazy_match! igoal with
+  lazy_match! get_iris_goal () with
   | bi_wand ?h _ =>
       lazy_match! h with
       | ⌜True⌝%I => iIntros "_"
