rocq-osiris/theories/tactics/iris_bindings.v
@@ -1,0 +1,61 @@
+From iris.proofmode Require Import proofmode environments ltac_tactics.
+
+From Ltac2 Require Import Ltac2.
+
+(* -------------------------------------------------------------------------- *)
+
+(** *Ltac2 bindings for Iris Proofmode tactics *)
+
+Ltac2 iapply (lem : constr) (sel : constr option) :=
+  match sel with
+  | None => ltac1:(lem |- iApply lem) (Ltac1.of_constr lem)
+  | Some sel =>
+      ltac1:(lem sel |- iApply (lem with sel))
+              (Ltac1.of_constr lem) (Ltac1.of_constr sel)
+  end.
+
+Ltac2 Notation "iApply" "(" lem(open_constr) "with" sel(constr) ")" := iapply lem (Some sel).
+Ltac2 Notation "iApply" lem(open_constr) := iapply lem None.
+
+Ltac2 iintros (pat : constr) :=
+  ltac1:(pat |- iIntros pat) (Ltac1.of_constr pat).
+
+Ltac2 Notation "iIntros" pat(constr) := iintros pat.
+
+Ltac2 iframe (sel : constr option) :=
+  match sel with
+  | None => ltac1:(iFrame)
+  | Some sel => ltac1:(sel |- iFrame sel) (Ltac1.of_constr sel)
+  end.
+Ltac2 Notation "iFrame" := iframe None.
+Ltac2 Notation "iFrame" sel(constr) := iframe (Some sel).
+
+Ltac2 iSplit () := ltac1:(iSplit).
+Ltac2 Notation "iSplit" := iSplit ().
+
+Ltac2 iSplitL (selpat : constr) := ltac1:(selpat |- iSplitL selpat) (Ltac1.of_constr selpat).
+Ltac2 Notation "iSplitL" pat(constr) := iSplitL pat.
+
+Ltac2 iSplitR (selpat : constr) := ltac1:(selpat |- iSplitR selpat) (Ltac1.of_constr selpat).
+Ltac2 Notation "iSplitR" pat(constr) := iSplitR pat.
+
+Ltac2 iDestruct (lem : constr) (pat : constr) :=
+  ltac1:(lem pat |- iDestruct (lem) as pat)
+    (Ltac1.of_constr lem) (Ltac1.of_constr pat).
+Ltac2 Notation "iDestruct" "(" lem(constr) ")" "as" pat(constr) := iDestruct lem pat.
+
+Ltac2 iRevert (h : constr) :=
+  ltac1:(h |- iRevert h) (Ltac1.of_constr h).
+Ltac2 Notation "iRevert" h(constr) := iRevert h.
+
+Ltac2 iPureIntro () := ltac1:(iPureIntro).
+Ltac2 Notation "iPureIntro" := iPureIntro ().
+
+Ltac2 iStartProof () := ltac1:(iStartProof).
+Ltac2 Notation "iStartProof" := iStartProof ().
+
+Ltac2 iModIntro () := ltac1:(iModIntro).
+Ltac2 Notation "iModIntro" := iModIntro ().
+
+Ltac2 iAssumption () := ltac1:(iAssumption).
+Ltac2 Notation "iAssumption" := iAssumption ().
