rocq-osiris/theories/tactics/tactics.v
@@ -1,0 +1,1 @@
+From osiris.tactics Require Export utils iris_bindings.
