rocq-osiris/theories/tactics/utils.v
@@ -1,0 +1,85 @@
+From Ltac2 Require Import Ltac2 Printf.
+
+(* [all] takes a tactic and applies it to all subgoals. *)
+
+Ltac2 all (tac : unit -> unit) :=
+  Control.extend [] tac [].
+
+(* [last] applies a tactic to the last subgoal. *)
+
+Ltac2 last tac := Control.extend [] (fun _ => ()) [tac].
+
+(* [first] applies a tactic to the first subgoal. *)
+
+Ltac2 first tac := Control.extend [tac] (fun _ => ()) [].
+
+(* [try_complete] takes a tactic and either
+   solves the goal by running it or does nothing. *)
+
+Ltac2 try_complete (tac : unit -> unit) :=
+  Control.plus (fun _ => complete tac) (fun _ => ()).
+
+From iris Require Import base environments.
+From stdpp Require Import stringmap.
+
+(* [get_iris_goal] returns the current iris goal. *)
+
+Ltac2 get_iris_goal () :=
+  lazy_match! goal with
+  | [ |- envs_entails ?_envs ?goal ] => goal
+  | [ |- _ ] => Control.zero (Tactic_failure (Some (fprintf "Expected an iris goal")))
+  end.
+
+(* [get_iris_hyps] returns a tuple of iris environments [(Δi, Δs)], where
+   [Δi] is the intuitionistic environment, and
+   [Δs] is the spatial environment. *)
+
+Ltac2 get_iris_hyps () :=
+  lazy_match! goal with
+  | [ |- envs_entails ?envs ?_goal ] =>
+      match! envs with
+      | (Envs ?Δi ?Δs _) => (Δi, Δs)
+      end
+  | [ |- _ ] => Control.zero (Tactic_failure (Some (fprintf "Expected an iris goal")))
+  end.
+
+(* [idents_to_strings Δ] takes a list of iris hypothesis identifiers, and returns
+   the list of names of those hypotheses. *)
+
+Fixpoint idents_to_strings (Δ : list ident) : list string :=
+  match Δ with
+  | [] => []
+  | (IAnon _ :: Δ) => idents_to_strings Δ
+  | (INamed s :: Δ) => s :: idents_to_strings Δ
+  end.
+
+(* Takes a Rocq string as a base, returns a Rocq string that does not
+   clash with any name of a current iris hypothesis. *)
+
+Ltac2 iFresh' (h : constr) :=
+  lazy_match! goal with
+  | [ |- envs_entails ?Δ _ ] =>
+      let hs := eval cbv in (idents_to_strings (envs_dom $Δ)) in
+        eval vm_compute in (fresh_string_of_set $h (list_to_set $hs))
+  end.
+
+Ltac2 Notation "iFresh" := iFresh' '"~".
+Ltac2 Notation "iFresh" h(constr) := iFresh' h.
+
+(* Given a constr of the form [▷^n c] (where [n] might equal 0),
+   [strip_laters] returns [c]. *)
+
+Ltac2 rec strip_laters (g : constr) :=
+  lazy_match! g with
+  | bi_later ?c => strip_laters c
+  | _ => g
+  end.
+
+(* Check if the spatial environment is empty. *)
+
+Ltac2 empty_spatial_env () :=
+  let (_, Δs) := get_iris_hyps () in
+  match! Δs with
+  | Enil => true
+  | _ => false
+  end.
